Completely drop the dependency of AC

PrimaryLogic/NoAC.lean
@@ -1,5 +1,7 @@
 import Mathlib.Data.Set.Lattice.Image
 import Mathlib.Data.List.Basic
+import Mathlib.Computability.Encoding
+import Mathlib.Logic.Encodable.Pi
 
 -- Rewrite theorems in Lean4 and Mathlib avoiding the axiom of choice.
 set_option linter.unusedDecidableInType false
@@ -160,3 +162,204 @@ theorem image_insert_eq' {f : α → β} {a : α} :
     · right; exact h2
 
 end Set
+
+namespace Nat
+open Lean Meta Simp
+lemma bodd_add_div2' : ∀ n, (bodd n).toNat + 2 * div2 n = n
+  | 0 => rfl
+  | succ n => by
+    simp only [bodd_succ, div2_succ, Nat.mul_comm]
+    refine Eq.trans ?_ (congr_arg succ (bodd_add_div2' n))
+    cases bodd n
+    · simp only [Bool.not_false, Bool.toNat_true, succ_eq_add_one,
+        cond_false, Bool.toNat_false, zero_add]
+      rw [add_comm, mul_comm]
+    · simp only [Bool.not_true, Bool.toNat_false, succ_eq_add_one,
+        cond_true, zero_add, Bool.toNat_true]
+      omega
+
+lemma div2_val' (n) : div2 n = n / 2 := by
+  refine Nat.eq_of_mul_eq_mul_left (by decide)
+    (Nat.add_left_cancel (Eq.trans ?_ (Nat.mod_add_div n 2).symm))
+  rw [mod_two_of_bodd, bodd_add_div2']
+
+private def IsSqrt (n q : ℕ) : Prop :=
+  q * q ≤ n ∧ n < (q + 1) * (q + 1)
+
+private lemma AM_GM : {a b : ℕ} → (4 * a * b ≤ (a + b) * (a + b))
+  | 0, _ => by rw [Nat.mul_zero, Nat.zero_mul]; exact zero_le _
+  | _, 0 => by rw [Nat.mul_zero]; exact zero_le _
+  | a + 1, b + 1 => by
+    simpa only [Nat.mul_add, Nat.add_mul, show (4 : ℕ) = 1 + 1 + 1 + 1 from rfl, Nat.one_mul,
+      Nat.mul_one, Nat.add_assoc, Nat.add_left_comm, Nat.add_le_add_iff_left]
+      using Nat.add_le_add_right (@AM_GM a b) 4
+
+lemma sqrt.iter_sq_le' (n guess : ℕ) : sqrt.iter n guess * sqrt.iter n guess ≤ n := by
+  unfold sqrt.iter
+  let next := (guess + n / guess) / 2
+  if h : next < guess then
+    simpa only [next, dif_pos h] using sqrt.iter_sq_le' n next
+  else
+    apply Nat.mul_le_of_le_div
+    simp only [dite_eq_ite]
+    split_ifs with h1 <;> omega
+
+protected theorem lt_of_mul_lt_mul_left' {a b c : Nat} (h : a * b < a * c) : b < c := by
+  induction a with
+  | zero => simp at h
+  | succ n h' =>
+    rw [←Nat.sub_pos_iff_lt, ←Nat.mul_sub, ←Nat.ne_zero_iff_zero_lt,
+      Nat.mul_ne_zero_iff, Nat.sub_ne_zero_iff_lt] at h
+    exact h.2
+
+lemma sqrt.lt_iter_succ_sq' (n guess : ℕ) (hn : n < (guess + 1) * (guess + 1)) :
+    n < (sqrt.iter n guess + 1) * (sqrt.iter n guess + 1) := by
+  unfold sqrt.iter
+  -- m was `next`
+  let m := (guess + n / guess) / 2
+  dsimp
+  split_ifs with h
+  · suffices n < (m + 1) * (m + 1) by
+      simpa only [dif_pos h] using sqrt.lt_iter_succ_sq' n m this
+    refine Nat.lt_of_mul_lt_mul_left' ?_ (a := 4 * (guess * guess))
+    apply Nat.lt_of_le_of_lt AM_GM
+    rw [show (4 : ℕ) = 2 * 2 from rfl]
+    rw [Nat.mul_mul_mul_comm 2, Nat.mul_mul_mul_comm (2 * guess)]
+    refine Nat.mul_self_lt_mul_self (?_ : _ < _ * ((_ / 2) + 1))
+    rw [← add_div_right _ (by decide), Nat.mul_comm 2, Nat.mul_assoc,
+      show guess + n / guess + 2 = (guess + n / guess + 1) + 1 from rfl]
+    have aux_lemma {a : ℕ} : a ≤ 2 * ((a + 1) / 2) := by omega
+    refine lt_of_lt_of_le ?_ (Nat.mul_le_mul_left _ aux_lemma)
+    rw [Nat.add_assoc, Nat.mul_add]
+    exact Nat.add_lt_add_left (lt_mul_div_succ _ (lt_of_le_of_lt (Nat.zero_le m) h)) _
+  · exact hn
+
+protected theorem pow_le_pow_iff_right' {a n m : Nat} (h : 1 < a) :
+    a ^ n ≤ a ^ m ↔ n ≤ m := by
+  constructor
+  · apply Decidable.by_contra
+    intro w
+    simp only [Decidable.not_imp_iff_and_not, not_le] at w
+    apply Nat.lt_irrefl (a ^ n)
+    exact Nat.lt_of_le_of_lt w.1 (Nat.pow_lt_pow_of_lt h w.2)
+  · intro w
+    cases Nat.eq_or_lt_of_le w
+    case inl eq => subst eq; apply Nat.le_refl
+    case inr lt => exact Nat.le_of_lt (Nat.pow_lt_pow_of_lt h lt)
+
+private lemma sqrt_isSqrt (n : ℕ) : IsSqrt n (sqrt n) := by
+  match n with
+  | 0 => simp only [IsSqrt, sqrt, _root_.zero_le, ↓reduceIte, mul_zero,
+    Std.le_refl, zero_add, mul_one, zero_lt_one, and_self]
+  | 1 => simp only [IsSqrt, sqrt, Std.le_refl, ↓reduceIte, mul_one, true_and]; decide
+  | n + 2 =>
+    have h : ¬ (n + 2) ≤ 1 := by simp only [reduceLeDiff, not_false_eq_true]
+    simp only [IsSqrt, sqrt, h, ite_false]
+    refine ⟨sqrt.iter_sq_le' _ _, sqrt.lt_iter_succ_sq' _ _ ?_⟩
+    simp only [Nat.mul_add, Nat.add_mul, Nat.one_mul, Nat.mul_one, ← Nat.add_assoc]
+    rw [Nat.lt_add_one_iff, Nat.add_assoc, ← Nat.mul_two]
+    refine le_trans (Nat.le_of_eq (div_add_mod' (n + 2) 2).symm) ?_
+    rw [show (n + 2) / 2 * 2 + (n + 2) % 2 = n + 2 by omega]
+    simp only [shiftLeft_eq, Nat.one_mul]
+    refine Nat.le_of_lt (Nat.le_trans lt_log2_self (le_add_right_of_le ?_))
+    rw [←Nat.pow_add, Nat.pow_le_pow_iff_right' (by decide)]
+    conv =>
+      rhs; rw [add_assoc]
+      conv => rhs; rw [←add_assoc, add_comm, ←add_assoc, add_comm]
+      repeat rw [←add_assoc]
+    rw [Nat.add_le_add_iff_right]
+    omega
+
+lemma lt_succ_sqrt'' (n : ℕ) : n < succ (sqrt n) * succ (sqrt n) := (sqrt_isSqrt n).right
+lemma sqrt_le'' (n : ℕ) : sqrt n * sqrt n ≤ n := (sqrt_isSqrt n).left
+
+lemma sqrt_le_add' (n : ℕ) : n ≤ sqrt n * sqrt n + sqrt n + sqrt n := by
+  rw [←succ_mul]; exact le_of_lt_succ (lt_succ_sqrt'' n)
+
+theorem pair_unpair' (n : ℕ) : pair (unpair n).1 (unpair n).2 = n := by
+  dsimp only [unpair]; let s := sqrt n
+  have sm : s * s + (n - s * s) = n := Nat.add_sub_cancel' (sqrt_le'' _)
+  split_ifs with h
+  · simp [s, pair, h, sm]
+  · have hl : n - s * s - s ≤ s := Nat.sub_le_iff_le_add.2
+      (Nat.sub_le_iff_le_add'.2 <| by rw [← Nat.add_assoc]; apply sqrt_le_add')
+    simp [s, pair, hl.not_gt, Nat.add_assoc, Nat.add_sub_cancel' (le_of_not_gt h), sm]
+
+lemma le_sqrt'' {m n} : m ≤ sqrt n ↔ m * m ≤ n :=
+  ⟨fun h ↦ le_trans (mul_self_le_mul_self h) (sqrt_le'' n),
+    fun h ↦ le_of_lt_succ <| Nat.mul_self_lt_mul_self_iff.1 <| lt_of_le_of_lt h (lt_succ_sqrt'' n)⟩
+lemma sqrt_lt'' {m n} : sqrt m < n ↔ m < n * n := by simp only [← not_le, le_sqrt'']
+
+lemma sqrt_add_eq'' {a : Nat} (n : ℕ) (h : a ≤ n + n) : sqrt (n * n + a) = n :=
+  le_antisymm
+    (le_of_lt_succ <| sqrt_lt''.2 <| by
+      rw [mul_succ, succ_mul, add_assoc, Nat.add_lt_add_iff_left, add_succ, Nat.lt_succ_iff]
+      exact h)
+    (le_sqrt''.2 <| Nat.le_add_right ..)
+
+theorem unpair_pair' (a b : ℕ) : unpair (pair a b) = (a, b) := by
+  dsimp only [pair]; split_ifs with h
+  · show unpair (b * b + a) = (a, b)
+    have be : sqrt (b * b + a) = b := sqrt_add_eq'' _ (le_trans (le_of_lt h) (Nat.le_add_left _ _))
+    simp only [unpair, be]
+    split_ifs with h1
+    · congr; omega
+    · congr
+      · omega
+      · omega
+  · show unpair (a * a + a + b) = (a, b)
+    have ae : sqrt (a * a + (a + b)) = a := by
+      rw [sqrt_add_eq'']
+      exact Nat.add_le_add_left (le_of_not_gt h) _
+    simp only [unpair, Nat.add_assoc, ae]
+    split_ifs with h1
+    · congr
+      · omega
+      · omega
+    · congr; omega
+
+theorem unpair_right_le' (n : ℕ) : (unpair n).2 ≤ n := by
+  simpa only [pair_unpair'] using right_le_pair n.unpair.1 n.unpair.2
+
+end Nat
+
+namespace Encodable
+variable {α : Type u} [Encodable α]
+
+instance Sum.encodable' {β} [Encodable β] : Encodable (α ⊕ β) :=
+  ⟨encodeSum, decodeSum, fun s => by cases s <;>
+  simp [encodeSum, Nat.div2_val', decodeSum, encodek]⟩
+
+open Nat in
+def decodeList' : ℕ → Option (List α)
+  | 0 => some []
+  | succ v =>
+    match unpair v, unpair_right_le' v with
+    | (v₁, v₂), h =>
+      have : v₂ < succ v := lt_succ_of_le h
+      (· :: ·) <$> decode (α := α) v₁ <*> decodeList' v₂
+
+theorem decodeList_encodeList_eq_self' (l : List α) : decodeList' (encodeList l) = some l := by
+  induction l <;> simp only [encodeList, Nat.succ_eq_add_one, decodeList', Nat.unpair_pair',
+    encodek, Option.map_eq_map, Option.map_some, Option.seq_some, *]
+
+instance List.encodable' : Encodable (List α) :=
+  ⟨encodeList, decodeList', decodeList_encodeList_eq_self'⟩
+
+instance Sigma.encodable' {γ} [(a : α) → Encodable (γ a)] : Encodable (Sigma γ) :=
+  ⟨encodeSigma, decodeSigma, fun ⟨a, b⟩ => by
+    simp only [decodeSigma, encodeSigma, Nat.unpair_pair',
+      encodek, Option.bind_some, Option.map_some]⟩
+
+instance List.Vector.encodable' [Encodable α] {n} : Encodable (List.Vector α n) :=
+  inferInstanceAs <| Encodable (Subtype _)
+
+instance finArrow' [Encodable α] {n} : Encodable (Fin n → α) :=
+  ofEquiv _ (Equiv.vectorEquivFin _ _).symm
+
+instance finPi' (n) (π : Fin n → Type*) [∀ i, Encodable (π i)] : Encodable (∀ i, π i) :=
+  ofEquiv _ (Equiv.piEquivSubtypeSigma (Fin n) π)
+
+instance Bool.encodable' : Encodable Bool :=
+  ofEquiv (Unit ⊕ Unit) Equiv.boolEquivPUnitSumPUnit
+end Encodable
